CpcMini/Logos.lean
@@ -180,8 +180,6 @@ inductive Proof : Type where
 
 /- Definition of Eunoia signature -/
 
-
-
 mutual
 
 def __eo_mk_apply : Term -> Term -> Term
@@ -282,19 +280,6 @@ def __mk_symm : Term -> Term
 
 def __eo_prog_symm : Proof -> Term
   | (Proof.pf F) => (__mk_symm F)
-  | _ => Term.Stuck
-
-
-def __mk_trans : Term -> Term -> Term -> Term
-  | Term.Stuck , _ , _  => Term.Stuck
-  | _ , Term.Stuck , _  => Term.Stuck
-  | t1, t2, (Term.Apply (Term.Apply Term.and (Term.Apply (Term.Apply Term.eq t3) t4)) tail) => (__eo_requires t2 t3 (__mk_trans t1 t4 tail))
-  | t1, t2, (Term.Boolean true) => (Term.Apply (Term.Apply Term.eq t1) t2)
-  | _, _, _ => Term.Stuck
-
-
-def __eo_prog_trans : Proof -> Term
-  | (Proof.pf (Term.Apply (Term.Apply Term.and (Term.Apply (Term.Apply Term.eq t1) t2)) tail)) => (__mk_trans t1 t2 tail)
   | _ => Term.Stuck
 
 
@@ -429,9 +414,28 @@ def __eo_typeof : Term -> Term
   | _ => Term.Stuck
 
 
+end
+
+
+
+mutual
+
+def __mk_trans : Term -> Term -> Term -> Term
+  | Term.Stuck , _ , _  => Term.Stuck
+  | _ , Term.Stuck , _  => Term.Stuck
+  | t1, t2, (Term.Apply (Term.Apply Term.and (Term.Apply (Term.Apply Term.eq t3) t4)) tail) => (__eo_requires t2 t3 (__mk_trans t1 t4 tail))
+  | t1, t2, (Term.Boolean true) => (Term.Apply (Term.Apply Term.eq t1) t2)
+  | _, _, _ => Term.Stuck
+
+
+def __eo_prog_trans : Proof -> Term
+  | (Proof.pf (Term.Apply (Term.Apply Term.and (Term.Apply (Term.Apply Term.eq t1) t2)) tail)) => (__mk_trans t1 t2 tail)
+  | _ => Term.Stuck
 
 
 end
+
+
 
 /- Definition of the checker -/
 
